theories/GraphCore/TensorGraphFacts.v
@@ -1,0 +1,823 @@
+From QuantumLib Require Import Complex.
+Require Import Aux_pos.
+Require Import Tensor.
+From stdpp Require Import list fin_maps.
+From stdpp Require Import pmap gmap.
+Require Import TensorExprDBSyntax TensorExprDBSemantics.
+Require Import ZXCore.
+Require ZifyBool.
+Require Import TensorGraph.
+
+#[local] Coercion pos_to_nat_pred : positive >-> nat.
+
+(* FIXME: Move *)
+Lemma Forall_filter {A} (P Q : A -> Prop) `{HP : forall a, Decision (P a)}
+  (l : list A) :
+  Forall Q (filter P l) <-> Forall (fun a => P a -> Q a) l.
+Proof.
+  induction l; [now split; constructor|].
+  cbn.
+  case_decide as HPa.
+  - rewrite 2 Forall_cons, IHl. tauto.
+  - rewrite Forall_cons, IHl. tauto.
+Qed.
+
+Lemma fmap_const {A B} (l : list A) (b : B) :
+  const b <$> l = replicate (length l) b.
+Proof.
+  induction l; cbn; f_equal; assumption.
+Qed.
+
+Lemma lookup_gmaps_to_Pmap {A} (mi mo : gmap nat A) p :
+  gmaps_to_Pmap mi mo !! p =
+  match p with
+  | xH => None
+  | p~0 => mi !! (p:>nat)
+  | p~1 => mo !! (p:>nat)
+  end.
+Proof.
+  unfold gmaps_to_Pmap.
+  rewrite lookup_union.
+  destruct p.
+  - rewrite (lookup_kmap_None _ _ _).2 by now cbn; lia.
+    rewrite option_union_left_id.
+    replace p~1 with ((bcons true ∘ Pos.of_succ_nat) p) by now cbn; lia.
+    rewrite lookup_kmap by apply _.
+    reflexivity.
+  - replace p~0 with ((bcons false ∘ Pos.of_succ_nat) p) by now cbn; lia.
+    rewrite lookup_kmap by apply _.
+    rewrite (lookup_kmap_None _ _ _).2 by now cbn; lia.
+    rewrite option_union_right_id.
+    reflexivity.
+  - rewrite 2 (lookup_kmap_None _ _ _).2 by now cbn; lia.
+    reflexivity.
+Qed.
+
+Lemma length_list_filter_ext {A B} (P : A -> Prop) (Q : B -> Prop)
+  `{HP : forall a, Decision (P a)} `{HQ : forall b, Decision (Q b)}
+  (l : list A) (l' : list B) :
+  Forall2 (λ a b, P a <-> Q b) l l' ->
+  length (filter P l) = length (filter Q l').
+Proof.
+  intros Hall.
+  induction Hall; [reflexivity|].
+  cbn.
+  unshelve (erewrite decide_ext by eassumption); [auto|].
+  case_decide; cbn; f_equal; easy.
+Qed.
+
+(* FIXME: Move *)
+Lemma lengthN_fmap {A B} (f : A -> B) (l : list A) :
+  lengthN (f <$> l) = lengthN l.
+Proof.
+  apply lengthN_eq, length_fmap.
+Qed.
+Lemma ppermute_fmap {A B} p (f : A -> B) (l : list A) :
+  ppermute p (f <$> l) = f <$> ppermute p l.
+Proof.
+  destruct (ppermute_case p l) as [(Hbdd & Hsome) | (Hndbb & Hnone)].
+  - apply (list_eq_same_length _ _ _ eq_refl);
+    [now rewrite length_fmap, 2 length_ppermute, length_fmap|].
+    intros i x y.
+    rewrite length_fmap, length_ppermute.
+    intros Hi.
+    rewrite lookup_ppermute_alt_bdd by now rewrite ?lengthN_fmap, ?length_fmap.
+    rewrite 2 list_lookup_fmap.
+    rewrite lookup_ppermute_alt_bdd by easy.
+    congruence.
+  - now rewrite 2 ppermute_not_bdd by now rewrite ?lengthN_fmap.
+Qed.
+Lemma default_is_Some_ext_mor_gen {B} {R : relation B} (d d' : B)
+  (mb mb' : option B) : R d d' ->
+  (forall b, mb = Some b -> mb' = None -> R b d') ->
+  (forall b', mb = None -> mb' = Some b' -> R d b') ->
+  (forall b b', mb = Some b -> mb' = Some b' -> R b b') ->
+  R (default d mb) (default d' mb').
+Proof.
+  destruct mb, mb'; cbn; eauto.
+Qed.
+Lemma default_is_Some_ext_mor {B} {R : relation B} (d d' : B)
+  (mb mb' : option B) :
+  (is_Some mb <-> is_Some mb') ->
+  R d d' ->
+  (forall b b', mb = Some b -> mb' = Some b' -> R b b') ->
+  R (default d mb) (default d' mb').
+Proof.
+  intros HSome Hd HR.
+  rewrite 2 is_Some_alt in HSome.
+  destruct mb, mb'; cbn; naive_solver.
+Qed.
+Lemma not_elem_of_list_fmap {A B} (f : A -> B) (l : list A) (b : B) :
+  b ∉ f <$> l <-> forall a, a ∈ l -> f a ≠ b.
+Proof.
+  rewrite elem_of_list_fmap.
+  naive_solver.
+Qed.
+Lemma Permutation_swap_app_app {A} (l1 l2 l3 l4 : list A) :
+  (l1 ++ l2) ++ (l3 ++ l4) ≡ₚ (l1 ++ l3) ++ (l2 ++ l4).
+Proof.
+  solve_Permutation.
+Qed.
+Lemma forall_var (P : var -> Prop) :
+  (forall v, P v) <-> (forall r, P (rel r)) /\ (forall l, P (loc l)) /\
+    (forall g, P (glob g)).
+Proof.
+  split; [auto|].
+  now intros (?&?&?) [].
+Qed.
+Lemma and_is_True_r {P Q} : Q -> P /\ Q <-> P.
+Proof. tauto. Qed.
+Lemma and_is_True_l {P Q} : P -> P /\ Q <-> Q.
+Proof. tauto. Qed.
+Lemma and_or_distr_r {P Q R} : (P \/ Q) /\ R <-> P /\ R \/ Q /\ R.
+Proof. tauto. Qed.
+Lemma and_or_distr_l {P Q R} : P /\ (Q \/ R) <-> P /\ Q \/ P /\ R.
+Proof. tauto. Qed.
+Lemma iff_True {P} : (P <-> True) <-> P.
+Proof. tauto. Qed.
+Lemma iff_True_1 {P} : P -> (P <-> True).
+Proof. tauto. Qed.
+Lemma iff_True_2 {P} : (P <-> True) -> P.
+Proof. tauto. Qed.
+
+
+
+
+
+
+
+Definition mk_tg {R A} (tm : TensorMap R A) (es : EdgeSet) : TensorGraph :=
+  (tm, es).
+
+
+Section TensorGraphFacts.
+
+Context {R : Type} {A : Type}.
+
+Context `{SR : SemiRing R rO rI radd rmul req}.
+
+(* Notation "0" := rO.
+Notation "1" := rI. *)
+Notation "x '==' y" := (req x y) (at level 70).
+Infix "+" := radd.
+Infix "*" := rmul.
+
+Add Ring R : SR.(RSRth)
+  (setoid SR.(Req_equiv) SR.(Req_ext)).
+
+Let Req_equivalence : Equivalence req := Req_equiv.
+Local Existing Instance Req_equivalence.
+
+Let Radd_proper := Req_ext.(SRadd_ext) : Proper (req ==> req ==> req) radd.
+Local Existing Instance Radd_proper.
+
+Let Rmul_proper := Req_ext.(SRmul_ext) : Proper (req ==> req ==> req) rmul.
+Local Existing Instance Rmul_proper.
+
+
+
+
+Let TensorGraph := @TensorGraph R A.
+
+Definition graph_tabs (tg : TensorGraph) : abstypecontext :=
+  kmap (Pos.of_succ_nat) $
+    map_imap (fun n (dt : DimensionlessTensor _) =>
+    let node := mk_node tg n in
+    let inarity := length node.1.2 in
+    let outarity := length node.2 in
+    Some (replicate (inarity + outarity) 0)) tg.1.
+
+Definition graph_tl (tg : TensorGraph) : vartypecontext :=
+  (gmaps_to_Pmap (set_to_map (fun k => (k, 0)) (inputs tg))
+    (set_to_map (fun k => (k, 0)) (outputs tg))).
+
+Definition graph_type_context (tg : TensorGraph) : typecontext :=
+  mk_tc (graph_tabs tg) ∅ (graph_tl tg) [].
+
+
+
+Lemma graph_semantics_WT tg :
+  well_typed (graph_type_context tg) (graph_tensorlist_semantics tg).
+Proof.
+  apply tl_well_typed_correct.
+  cbn.
+  unfold tl_well_typed_aux.
+  rewrite 2 Forall_fmap, Forall_forall.
+  intros (n & dt) Hn%elem_of_map_to_list.
+  cbn.
+  unfold graph_tabs.
+  rewrite lookup_kmap by apply _.
+  rewrite map_lookup_imap, Hn.
+  cbn.
+  f_equal.
+  rewrite !length_app, !length_fmap.
+  apply (list_eq_same_length _ _ _ eq_refl).
+  - rewrite !length_fmap, !length_app, !length_fmap, length_replicate.
+    reflexivity.
+  - rewrite !length_fmap, !length_app, !length_fmap.
+    intros i x y Hi.
+    rewrite list_lookup_fmap.
+    destruct (replicate _ _ !! _) as [ri|] eqn:Hri; [|easy].
+    apply lookup_replicate in Hri as [-> _].
+    cbn.
+    intros [= <-].
+    intros Hhyp; symmetry; revert Hhyp.
+    refine ((Forall_lookup (.= Some 0) _).1 _ i y).
+    rewrite Forall_fmap.
+    rewrite 3 Forall_app, 4 ! Forall_fmap.
+    unfold compose; cbn.
+    rewrite 4 Forall_filter.
+    unfold i_internal_edges, i_external_edges.
+    rewrite app_nil_r.
+    split; (split; apply Forall_forall; intros (k, e) Hke%elem_of_enumerate;
+      intros [= Hen];
+
+      [rewrite <- fmap_reverse; rewrite list_lookup_fmap;
+        rewrite pos_to_nat_pred_of_nat; cbn;
+        destruct (reverse _  !! k) as [v|] eqn:Hv; [easy|
+        apply lookup_lt_Some in Hke;
+        apply lookup_ge_None in Hv;
+        rewrite length_reverse in Hv; lia]|]);
+    unfold graph_tl; rewrite lookup_gmaps_to_Pmap, lookup_set_to_map by easy;
+    [exists e.1|exists e.2]; (split; [|cbn; f_equal; lia]).
+    + unfold inputs.
+      rewrite elem_of_filter, elem_of_list_to_set.
+      apply elem_of_list_lookup_2 in Hke.
+      unfold external_edges in Hke.
+      apply elem_of_list_filter in Hke.
+      pose proof (mk_is_Some _ _ Hn : is_key tg n) as Hkey.
+      unfold not_internal, is_internal in Hke.
+      split; [subst; tauto|].
+      now apply elem_of_list_fmap_1.
+    + unfold outputs.
+      rewrite elem_of_filter, elem_of_list_to_set.
+      apply elem_of_list_lookup_2 in Hke.
+      unfold external_edges in Hke.
+      apply elem_of_list_filter in Hke.
+      pose proof (mk_is_Some _ _ Hn : is_key tg n) as Hkey.
+      unfold not_internal, is_internal in Hke.
+      split; [subst; tauto|].
+      now apply elem_of_list_fmap_1.
+Qed.
+
+Context `{Summable A}.
+
+Definition num_internals (tg : TensorGraph) : nat :=
+  length (filter (is_internal tg) tg.2).
+
+Definition num_externals (tg : TensorGraph) : nat :=
+  length (filter (not_internal tg) tg.2).
+
+Lemma fold_num_internals' tm es es' :
+  length (filter (is_internal (mk_tg tm es')) es) =
+  num_internals (mk_tg tm es).
+Proof. reflexivity. Qed.
+
+Definition abs_length_eq {A} : relation (Idx * list A * list A) :=
+  fun '(f, low, up) '(f', low', up') =>
+  f = f' /\ length low = length low' /\ length up = length up'.
+
+Lemma mk_node_perm_eq_lengths (tm : TensorMap R A) es es' k :
+  es ≡ₚ es' ->
+  length (mk_node (mk_tg tm es) k).1.2 =
+  length (mk_node (mk_tg tm es') k).1.2 /\
+  length (mk_node (mk_tg tm es) k).2 =
+  length (mk_node (mk_tg tm es') k).2.
+Proof.
+  intros Hes.
+  cbn.
+  change (is_internal (mk_tg tm es')) with (is_internal (mk_tg tm es)).
+  change (not_internal (mk_tg tm es')) with (not_internal (mk_tg tm es)).
+  rewrite 4 length_app.
+  split; f_equal; rewrite 2 length_fmap;
+      (rewrite <- (length_fmap snd);
+      (change (λ e : Ty * (Ty * Ty), e.2.2 = k) with
+        ((λ e : Ty * Ty, e.2 = k) ∘ @snd Ty _) ||
+        change (λ e : Ty * (Ty * Ty), e.2.1 = k) with
+        ((λ e : Ty * Ty, e.1 = k) ∘ @snd Ty _));
+      etransitivity; [symmetry; apply (f_equal length);
+        refine (list_filter_fmap snd _)|];
+      rewrite fmap_imap; unfold compose at 1; cbn -[compose];
+      rewrite imap_to_fmap, list_fmap_id;
+
+      (* rewrite imap_snds by (now rewrite length_fmap, length_seq); *)
+      rewrite <- (length_fmap (@snd _ (_*_)));
+      etransitivity; [|apply (f_equal length);
+        refine (list_filter_fmap snd _)];
+      rewrite fmap_imap; unfold compose at 1; cbn -[compose];
+      rewrite imap_to_fmap, list_fmap_id);
+    rewrite <- Hes;
+    reflexivity.
+Qed.
+
+
+
+
+
+
+(*
+Lemma mk_node_perm_eq (tm : TensorMap R A) es es' fint fext k :
+  posperm (lengthP (filter (is_internal (mk_tg tm es)) es)) fint ->
+  ppermute fint (filter (is_internal (mk_tg tm es)) es) =
+  filter (is_internal (mk_tg tm es')) es' ->
+
+  posperm (lengthP (filter (not_internal (mk_tg tm es')) es')) fext ->
+  ppermute fext (filter (not_internal (mk_tg tm es)) es) =
+  filter (not_internal (mk_tg tm es')) es' ->
+  abs_perm
+    ((mk_node (mk_tg tm es) k))
+    (relabel_abs (var_map fint fext Datatypes.id) (mk_node (mk_tg tm es') k)).
+Proof.
+  intros Hfint Hfint_pperm Hfext Hfext_pperm.
+  cbn.
+  split; [reflexivity|].
+  rewrite 2 fmap_app.
+  split; f_equiv.
+  - apply posperm_imap_eq' in Hfint as Hfint'.
+    unfold EdgeSet in *.
+    setoid_rewrite Hfint'.
+    rewrite ppermute_permutation. 2:{
+      rewrite lengthN_correct_rev, length_zip, length_fmap,
+        length_seq, length_ppermute, Nat.min_id, <- lengthN_correct_rev.
+      now apply posperm_inv_posperm.
+    }
+    setoid_rewrite <- Hfint_pperm.
+    rewrite posperm_imap_eq by easy.
+    symmetry.
+    rewrite ppermute_permutation. 2:{
+      now rewrite lengthN_correct_rev, length_zip, length_fmap,
+        length_seq, Nat.min_id, <- lengthN_correct_rev.
+    }
+    rewrite zip_with_ppermute_r by now
+      rewrite ?lengthN_correct_rev, length_fmap, length_seq,
+        <- ?lengthN_correct_rev.
+
+
+    apply eq_reflexivity.
+
+
+    apply list_eq_Forall2.
+    rewrite 2 Forall2_fmap_l, Forall2_fmap_r.
+    apply Forall2
+
+
+
+
+
+
+
+    symmetry.
+    rewrite lengthN_correct_rev, length_fmap, length_seq, <- lengthN_correct_rev.
+    symmetry.
+
+    apply (list_eq_same_length _ _ _ eq_refl). 1:{
+      rewrite !length_fmap.
+      rewrite <- (length_fmap snd).
+      change (@filter (Ty * (Ty * Ty)) ?B ?H _) with
+        (@filter (Ty * (Ty * Ty)) B H ((λ e, e.2 = k) ∘ snd)).
+      etransitivity; [symmetry; apply (f_equal length);
+        refine (list_filter_fmap snd _)|].
+      rewrite snd_zip by now rewrite length_fmap, length_seq.
+      rewrite <- (length_fmap (@snd _ (_*_))).
+      etransitivity; [|apply (f_equal length);
+        refine (list_filter_fmap snd _)].
+      rewrite <- ppermute_fmap.
+      rewrite snd_zip by now rewrite length_ppermute, length_fmap, length_seq.
+      now rewrite ppermute_permutation by easy.
+    }
+
+    intros i x y Hi.
+    rewrite ! list_lookup_fmap.
+
+
+    rewrite <- list_fmap_compose.
+    unfold compose; cbn.
+    evar (n : nat);
+    replace (length _) with n. 2:{
+
+      rewrite length_fmap.
+      rewrite <- (length_fmap snd).
+      change (@filter (Ty * (Ty * Ty)) ?B ?H _) with
+        (@filter (Ty * (Ty * Ty)) B H ((λ e, e.2 = k) ∘ snd)).
+      etransitivity; [|apply (f_equal length);
+        refine (list_filter_fmap snd _)].
+      rewrite snd_zip by now rewrite length_fmap, length_seq, length_ppermute.
+      rewrite ppermute_permutation by easy.
+      unfold n; reflexivity.
+    }
+    subst n.
+    intros i x y Hi.
+    rewrite 2 list_lookup_fmap.
+
+    list_lookup filter
+
+  intros Hes.
+  cbn.
+  rewrite !length_app, !length_fmap.
+  split; f_equal.
+
+  erewrite <- (length_fmap snd).
+  epose proof (fun l => list_filter_fmap snd (P:= λ e, e.2 = k)
+    l) as Hrw.
+  etransitivity; [apply (f_equal length); symmetry; apply Hrw|].
+
+  rewrite <- Hrw.
+
+  1, 3: rewrite <- Hes at 2.
+  cbv delta [mk_node] beta.
+*)
+
+Lemma graph_mabs_perm_eq (tm : TensorMap R A) es es' :
+  es ≡ₚ es' ->
+  graph_mabs (mk_tg tm es) = graph_mabs (mk_tg tm es').
+Proof.
+  intros Hes.
+  unfold graph_mabs.
+  f_equal.
+  cbn [fst mk_tg].
+  apply map_imap_ext.
+  intros k.
+  apply option_fmap_ext.
+  intros dt.
+  f_equal.
+  pose proof (mk_node_perm_eq_lengths tm es es' k Hes) as (-> & ->).
+  reflexivity.
+Qed.
+
+Definition type {A} (a : A) : Type := A.
+Definition domtype {A B} (f : A -> B) : Type := A.
+Definition codomtype {A B} (f : A -> B) : Type := B.
+#[global] Arguments type /.
+#[global] Arguments domtype /.
+#[global] Arguments codomtype /.
+
+Ltac2 empty_flags () : Std.red_flags := {
+  Std.rStrength := Std.Norm;
+  Std.rBeta := Init.false;
+  Std.rMatch := Init.false;
+  Std.rFix := Init.false;
+  Std.rCofix := Init.false;
+  Std.rZeta := Init.false;
+  Std.rDelta := Init.false;
+  Std.rConst := [];
+}.
+
+Import Ltac2.Notations.
+
+Notation "'right_uncompose' fg g" :=
+  ((* let fpat :=  *)
+    ltac2:(
+      let fg := Constr.pretype fg in
+      let g := Constr.pretype g in  (* TODO: Improve with expected type from fg *)
+      let tf := match! Constr.type fg with
+        | ?a -> _ => a
+        end in
+      let res := Constr.in_context ident:(x) tf (fun () =>
+        let fg' := Std.eval_hnf fg in
+        let fgx := Std.eval_cbv {(empty_flags()) with Std.rBeta := Init.true}
+            '($fg' &x) in
+        let pat := Std.eval_pattern [('($g &x), Std.AllOccurrences)] fgx in
+        match! pat with
+        | ?f _ => exact $f
+        end) in
+      match Constr.Unsafe.kind res with
+      | Constr.Unsafe.Lambda _ body =>
+        ltac1:(r |- let r' := eval cbn in r in exact r') (Ltac1.of_constr body)
+      | _ => Control.throw (Init.Tactic_failure Init.None)
+      end
+        )) (at level 10, fg at level 0, g at level 0).
+
+(* Goal True.
+Check (right_uncompose (λ (x : nat * (nat * nat)), x.2.2) (@snd nat (nat * nat))). *)
+
+Lemma graph_semantics_abstracts_is_Some (tm : TensorMap R A) es mi mo k
+  (mr': Vlist graph_V (replicate (num_internals (mk_tg tm es)) 0))
+  (Hmr': WF_Vlist graph_V mr') :
+  k ∈ dom tm ->
+  is_Some
+  (join_list
+     (get_var graph_V ∅ (graph_ml mi mo) (reverse mr') <$>
+      ((mk_internal_var <$>
+        filter (λ e : Ty * (Ty * Ty), e.2.2 = k)
+          (imap pair
+             (filter (is_internal (mk_tg tm es)) es))) ++
+       (mk_external_var false <$>
+        filter (λ e : Ty * (Ty * Ty), e.2.2 = k)
+          (imap pair
+             (filter (not_internal (mk_tg tm es)) es)))) ++
+      (mk_internal_var <$>
+       filter (λ e : Ty * (Ty * Ty), e.2.1 = k)
+         (imap pair (filter (is_internal (mk_tg tm es)) es))) ++
+      (mk_external_var true <$>
+       filter (λ e : Ty * (Ty * Ty), e.2.1 = k)
+         (imap pair
+            (filter (not_internal (mk_tg tm es)) es))))
+   ≫= λ args : list (Vval graph_V),
+        graph_mabs (mk_tg tm es) !! Pos.of_succ_nat k
+        ≫= λ fval : Vfunc graph_V,
+             Vapplys graph_V fval args) <->
+  ((forall i, i ∈ (filter (λ e, e.2 = k /\ ~ is_key (mk_tg tm es) e.1) es).*1 ->
+    (i:>nat) ∈ dom mi) /\
+  (forall o, o ∈ (filter (λ e, e.1 = k /\ ~ is_key (mk_tg tm es) e.2) es).*2 ->
+    (o:>nat) ∈ dom mo)) /\ True.
+Proof.
+  intros Hkdom.
+  unfold graph_mabs.
+  rewrite lookup_kmap by apply _.
+  rewrite map_lookup_imap.
+  apply elem_of_dom in Hkdom as [fk Hfk].
+  cbn [fst mk_tg].
+  rewrite Hfk.
+  cbn [mbind option_bind].
+  rewrite bind_is_Some.
+  rewrite join_list_is_Some.
+  apply and_iff_from_l.
+  - rewrite not_elem_of_list_fmap.
+    rewrite <- Forall_forall.
+    rewrite Permutation_swap_app_app.
+    rewrite <- fmap_app.
+    change (mk_external_var false) with
+      (loc ∘ (λ e : Ty * (Ty * Ty), bcons false (Pos.of_succ_nat e.2.1))).
+    change (mk_external_var true) with
+      (loc ∘ (λ e : Ty * (Ty * Ty), bcons true (Pos.of_succ_nat e.2.2))).
+    rewrite 2 list_fmap_compose, <- fmap_app.
+    rewrite Forall_app.
+    rewrite and_is_True_l. 2:{
+      rewrite Forall_fmap, Forall_forall.
+      intros x.
+      rewrite elem_of_app, 2 elem_of_list_filter.
+      rewrite <- and_or_distr_r.
+      intros [Hxk (i & e & -> & Hlook)%elem_of_lookup_imap].
+      cbn.
+      apply not_eq_None_Some.
+      apply lookup_lt_is_Some.
+      rewrite length_reverse.
+      apply Forall2_length in Hmr' as Hlen.
+      unfold Vval.
+      rewrite <- Hlen, length_replicate.
+      unfold num_internals.
+      apply lookup_lt_Some in Hlook.
+      cbn; lia.
+    }
+    rewrite Forall_fmap.
+    rewrite Forall_app, 2 Forall_fmap.
+    unfold compose; cbn.
+    unfold graph_ml.
+    setoid_rewrite lookup_fmap.
+    setoid_rewrite lookup_gmaps_to_Pmap.
+    setoid_rewrite pos_to_nat_pred_of_nat.
+    f_equiv.
+    + change (Forall _ ?l) with
+        (Forall (((λ x : Ty,
+        @mk_Vval graph_V 0 <$> mi !! x ≠ None)∘ fst) ∘ snd) l) at 1.
+      rewrite <- Forall_fmap.
+      change (filter (H:=?H) _ ?l) with
+        (filter (H:=H) ((λ e, e.2 = k) ∘ snd) l) at 1.
+      remember (filter _ _).*2 as l eqn:Hl.
+      pose proof (eq_trans Hl (eq_sym (list_filter_fmap snd _))) as Hl'.
+      clear Hl.
+      subst l.
+      rewrite fmap_imap.
+      unfold compose at 2.
+      cbn.
+      rewrite imap_to_fmap, list_fmap_id.
+      rewrite <- Forall_fmap.
+      rewrite <- Forall_forall.
+      setoid_rewrite list_filter_filter.
+      erewrite list_filter_iff; [apply Forall_iff|].
+      * intros x.
+        now rewrite not_eq_None_Some, fmap_is_Some, elem_of_dom.
+      * intros (i, j).
+        cbn.
+        unfold not_internal, is_internal.
+        cbn.
+        apply and_iff_from_l; [easy|].
+        intros -> _.
+        enough (is_key (mk_tg tm es) k) by tauto.
+        apply elem_of_dom.
+        refine (elem_of_dom_2 _ _ _ Hfk).
+    + change (Forall _ ?l) with
+        (Forall (((λ x : Ty,
+        @mk_Vval graph_V 0 <$> mo !! x ≠ None) ∘ snd) ∘ snd) l) at 1.
+      rewrite <- Forall_fmap.
+      change (filter (H:=?H) _ ?l) with
+        (filter (H:=H) ((λ e, e.1 = k) ∘ snd) l) at 1.
+      remember (filter _ _).*2 as l eqn:Hl.
+      pose proof (eq_trans Hl (eq_sym (list_filter_fmap snd _))) as Hl'.
+      clear Hl.
+      subst l.
+      rewrite fmap_imap.
+      unfold compose at 2.
+      cbn.
+      rewrite imap_to_fmap, list_fmap_id.
+      rewrite <- Forall_fmap.
+      rewrite <- Forall_forall.
+      setoid_rewrite list_filter_filter.
+      erewrite list_filter_iff; [apply Forall_iff|].
+      * intros x.
+        now rewrite not_eq_None_Some, fmap_is_Some, elem_of_dom.
+      * intros (i, j).
+        cbn.
+        unfold not_internal, is_internal.
+        cbn.
+        apply and_iff_from_l; [easy|].
+        intros -> _.
+        enough (is_key (mk_tg tm es) k) by tauto.
+        apply elem_of_dom.
+        refine (elem_of_dom_2 _ _ _ Hfk).
+  - intros Hnone_nin [Hmi Hmo].
+    apply iff_True_1.
+    intros vs Hvs%join_list_Some.
+    apply Vapplys_is_Some.
+    cbn -[mk_node].
+    apply (list_eq_same_length _ _ _ eq_refl).
+    1: {
+      apply (f_equal length) in Hvs.
+      rewrite 2 length_fmap in Hvs.
+      rewrite length_fmap, length_replicate.
+      unfold Vval in *.
+      rewrite <- Hvs.
+      cbn.
+      rewrite <- length_app.
+      reflexivity.
+    }
+    intros i x y Hi.
+    rewrite length_fmap in Hi.
+    rewrite lookup_replicate.
+    rewrite list_lookup_fmap.
+    intros [-> Hi'].
+    apply (f_equal (.!! i)) in Hvs.
+    rewrite ! list_lookup_fmap in Hvs.
+    unfold Vval in *.
+    destruct (vs !! i) as [vi|] eqn:Hvi in *; [|easy].
+    cbn.
+    intros [= <-].
+    symmetry.
+    cbn in Hvs.
+    rewrite fmap_Some in Hvs.
+    destruct Hvs as (v & Hv & HSvi).
+    change (projT1 vi) with (from_option projT1 0 (Some vi)).
+    rewrite HSvi.
+    apply elem_of_list_lookup_2 in Hv as Hin.
+    rewrite Permutation_swap_app_app, <- fmap_app in Hin.
+    rewrite 2 elem_of_app, 3 elem_of_list_fmap in Hin.
+    destruct Hin as [((n&?&?) & -> & Hin) |[((?&?&?) & -> & Hin) | ((?&?&?) & -> & Hin)]].
+    + cbn.
+      rewrite pos_to_nat_pred_of_nat.
+      destruct (reverse _ !! _) as [mr'i|] eqn:Hmr'i; [|easy].
+      apply elem_of_list_lookup_2 in Hmr'i as Hn.
+      pose proof Hmr' as HWF.
+      unfold WF_Vlist in HWF.
+      rewrite Forall2_lookup in HWF.
+      specialize (HWF (length mr' - S n)).
+      pose proof Hmr'i as Hmri.
+      rewrite reverse_lookup in Hmri by 
+        now apply lookup_lt_Some in Hmr'i; rewrite length_reverse in Hmr'i.
+      setoid_rewrite Hmri in HWF.
+      destruct (replicate _ _ !! _) as [ri|] eqn:Hrep in HWF; [|easy].
+      apply lookup_replicate in Hrep as [-> ?].
+      inversion HWF; subst.
+      cbn.
+      easy.
+    + cbn.
+      unfold graph_ml.
+      rewrite lookup_fmap.
+      destruct (_ !! _) in |- *; reflexivity.
+    + cbn.
+      unfold graph_ml.
+      rewrite lookup_fmap.
+      destruct (_ !! _) in |- *; reflexivity.
+Qed.
+
+
+Lemma num_internals_perm_eq tm es es' : es ≡ₚ es' ->
+  num_internals (mk_tg tm es) = num_internals (mk_tg tm es').
+Proof.
+  intros Hes.
+  unfold num_internals.
+  cbn.
+  rewrite <- Hes at 2.
+  reflexivity.
+Qed.
+
+(* 
+Lemma graph_semantics_perm_eq_aux (tm : TensorMap R A) es es' :
+  es ≡ₚ es' ->
+  forall mi mo,
+  graph_map_semantics (mk_tg tm es) mi mo ==
+  graph_map_semantics (mk_tg tm es') mi mo.
+Proof.
+  intros Hes mi mo.
+  cbn.
+  rewrite 2 fmap_const.
+  rewrite <- (graph_mabs_perm_eq tm es es' Hes).
+
+  change (is_internal (mk_tg tm es')) with (is_internal (mk_tg tm es)).
+  rewrite <- Hes at 1.
+  set (l := length _).
+  subst l.
+  rewrite fold_num_internals'.
+
+
+  apply tl_total_semantics_aux_ext_abs.
+
+  intros mr' Hmr'.
+
+  rewrite Forall2_fmap.
+  apply Forall_Forall2_diag.
+  rewrite Forall_forall.
+  intros k Hk.
+  rewrite rev_append_reverse, app_nil_r.
+  cbn.
+
+  apply default_is_Some_ext_mor; [|reflexivity|].
+  - assert (Hkdom : k ∈ dom tm) by now rewrite dom_alt, elem_of_list_to_set.
+
+    rewrite graph_semantics_abstracts_is_Some by easy.
+    rewrite (graph_mabs_perm_eq _ _ _ Hes).
+    rewrite graph_semantics_abstracts_is_Some; [..|easy]. 2:{
+      rewrite <- (num_internals_perm_eq _ _ _ Hes).
+      exact Hmr'.
+    }
+    f_equiv.
+    change (is_key (mk_tg tm es')) with (is_key (mk_tg tm es)).
+    f_equiv; apply forall_iff; intros ?.
+    f_equiv.
+    setoid_rewrite <- Hes.
+
+  f_equal.
+
+
+  induction Hes; [reflexivity|..].
+
+
+  setoid_rewrite fold_num_internals'.
+  rewrite <- Hes at 3.
+  rewrite fold_num_internals'.
+
+  rewrite 2 tl_total_semantics_aux_alt_Vlist.
+  setoid_rewrite rev_append_rev.
+  setoid_rewrite app_nil_r.
+
+
+  pose proof Hes as Hes'.
+
+  apply (filter_Permutation (is_internal (mk_tg tm es))) in Hes' as Hesint.
+
+  apply perm_exists_posperm in Hesint as Hf.
+  destruct Hf as (f & Hfperm & Hfppermute & Hlook).
+
+  eapply sum_of_relabel'_r2l with (ppermute f).
+  2:{
+    unfold sum_elements; cbn.
+    rewrite ppermute_posperm_permutes_Vlist_elements. 2:{
+      now rewrite lengthN_correct_rev, length_replicate, <- lengthN_correct_rev.
+    }
+    rewrite ppermute_replicate.
+    reflexivity.
+  }
+  intros ml Hml%elem_of_Vlist_elements.
+
+  apply tl_total_semantics_aux_ext_base_mr.
+  unshelve (instantiate (1:=_)).
+  unfold Vlist.
+  exact
+
+
+
+  eexists; cbn -[reverse].
+  rewrite !fmap_const.
+  rewrite reverse_replicate, lengthN_correct_rev, length_replicate.
+  replace (N.succ_pos _) with (Pos.of_succ_nat (num_internals (mk_tg tm es)))
+    by lia. *)
+
+(* 
+Lemma graph_semantics_perm_eq_aux (tm : TensorMap R A) es es' :
+  es ≡ₚ es' ->
+  forall mi mo,
+  graph_tensorlist_semantics (mk_tg tm es) =tl=
+  graph_tensorlist_semantics (mk_tg tm es').
+Proof.
+  intros Hes.
+  eexists; cbn -[reverse].
+  rewrite !fmap_const.
+  remember (num_internals (mk_tg tm es)) as x eqn:Hx.
+  pose proof Hx as Hx'.
+  cbn in Hx'.
+  rewrite <- Hx', Hx.
+  unfold is_internal, is_key in Hx' |- *.
+  cbn -[reverse num_internals] in Hx' |- *.
+  rewrite <- Hes at 1.
+  rewrite <- Hx', Hx.
+  clear x Hx Hx'.
+  rewrite reverse_replicate, lengthN_correct_rev, length_replicate.
+  replace (N.succ_pos _) with (Pos.of_succ_nat (num_internals (mk_tg tm es)))
+    by lia.
+  apply (filter_Permutation (is_internal (mk_tg tm es))) in Hes as Hesint.
+
+
+
+
+*)
+
+End TensorGraphFacts.
